Move back to CTL definitions quantifying over finite path prefixes

BinaryRelations.v
@@ -12,10 +12,18 @@ Notation "R ^*" := (clos_refl_trans _ R) (at level 35).
 Definition is_serial {A} (R: relation A) := forall a, exists b, R a b.
 Definition serial A := {R: relation A | is_serial R}.
 
-Definition is_serialT {A} (R: relation A) := forall a, {b | R a b}.
-Definition serialT A := {R: relation A & is_serialT R}.
+(* Definition is_serialT {A} (R: relation A) := forall a, {b | R a b}. *)
+(* Definition serialT A := {R: relation A & is_serialT R}. *)
+Definition serial_witness {A} (R: relation A) := forall a, {b | R a b}.
+Definition serialT A := {R: relation A & serial_witness R}.
 
 Definition reachable {A} (R: relation A) (l: list A) (b: A) := exists a, In a l /\ R^* a b.
+
+Definition is_serial_from {A} (R: relation A) s :=
+  forall s', R^* s s' -> exists s'', R s' s''.
+
+Definition serial_from_witness {A} (R: relation A) s :=
+  forall s', R^* s s' -> {s''| R s' s''}.
 
 Inductive steps : nat -> forall {A}, relation A -> relation A :=
   | steps_one   : forall {A} (R: relation A) x y,
