GeneralTactics.v
@@ -11,18 +11,16 @@ Ltac destructExists H id := destruct H as [id H].
 Ltac applyc H := apply H; clear H.
 Ltac eapplyc H := eapply H; clear H.
 
+Ltac specializec H x := specialize (H x); clear x.
+
 Ltac generalize_max := 
   repeat match goal with 
   | [H: _ |- _] => generalize dependent H
   end.
 
-Ltac generalize_max_except x :=
+Ltac max_induction x :=
   move x at top;
   generalize_max;
-  intro x.
-
-Ltac max_induction x :=
-  generalize_max_except x;
   induction x.
 
 Lemma reflect_N_compare: forall n m,
